Implemented unification

STLC/Id.v
@@ -1,5 +1,12 @@
-Require Import FSets OrderedTypeEx.
+Require Import Arith MSets.
 
-Definition t := nat.
+Module FSet := MSetList.Make (Nat_as_OT).
+Module FSetProperties := WProperties (FSet).
 
-Module FSet := FSetList.Make (Nat_as_OT).
+Definition t := FSet.E.t.
+Definition eq_dec := FSet.E.eq_dec.
+
+Hint Extern 1 (FSet.In _ (FSet.union _ _)) =>
+  apply FSet.union_spec.
+Hint Extern 1 (FSet.In _ (FSet.singleton _)) =>
+  apply FSet.singleton_spec.
