STLC/Types.v
@@ -1,6 +1,156 @@
+Require Import List Omega.
 Require Id.
 
 Inductive t :=
   | Bool
   | Fun : t -> t -> t
   | Var : Id.t -> t.
+
+Fixpoint FV t :=
+  match t with
+  | Bool => Id.FSet.empty
+  | Fun t1 t2 => Id.FSet.union (FV t1) (FV t2)
+  | Var x => Id.FSet.singleton x
+  end.
+
+Fixpoint size t :=
+  match t with
+  | Bool => 1
+  | Fun t1 t2 => 1 + size t1 + size t2
+  | Var _ => 1
+  end.
+
+Fixpoint subst x t0 t :=
+  match t with
+  | Bool => Bool
+  | Fun t1 t2 => Fun (subst x t0 t1) (subst x t0 t2)
+  | Var y =>
+      if Id.eq_dec x y then t0
+      else Var y
+  end.
+
+Definition eq_dec : forall t1 t2 : t, { t1 = t2 } + { t1 <> t2 }.
+Proof.
+  refine (fix eq_dec t1 t2 :=
+    match t1 as t1_ return { t1_ = t2 } + { t1_ <> t2 } with
+    | Bool =>
+        match t2 with
+        | Bool => left _
+        | _ => right _
+        end
+    | Fun t11 t12 =>
+        match t2 with
+        | Fun t21 t22 =>
+            if eq_dec t11 t21 then
+              if eq_dec t12 t22 then left _
+              else right _
+            else right _
+        | _ => right _
+        end
+    | Var x =>
+        match t2 with
+        | Var y =>
+            if Id.eq_dec x y then left _
+            else right _
+        | _ => right _
+        end
+    end); congruence.
+Qed.
+
+Lemma size_gt_0 : forall t,
+  0 < size t.
+Proof.
+  intros t.
+  destruct t; simpl in *; omega.
+Qed.
+
+Lemma subst_occur : forall x t1 t2,
+  Id.FSet.In x (FV (subst x t1 t2)) ->
+  Id.FSet.In x (FV t1).
+Proof.
+  intros x t1 t2 ?.
+  induction t2; simpl in *; eauto.
+  - destruct (Id.FSet.empty_spec H).
+  - apply Id.FSet.union_spec in H.
+    destruct H; eauto.
+  - destruct (Id.eq_dec x t0); simpl in *.
+    + eauto.
+    + eapply Id.FSet.singleton_spec in H.
+      congruence.
+Qed.
+
+Lemma subst_fv : forall x y t1 t2,
+  Id.FSet.In x (FV (subst y t1 t2)) ->
+  Id.FSet.In x (FV t1) \/ Id.FSet.In x (FV t2).
+Proof.
+  intros ? ? ? t2 ?.
+  induction t2; simpl in *; eauto.
+  - apply Id.FSet.union_spec in H.
+    destruct H as [ H | H ];
+    [ destruct (IHt2_1 H)
+    | destruct (IHt2_2 H) ]; eauto 9.
+  - destruct (Id.eq_dec y t0); eauto.
+Qed.
+
+Lemma subst_notin_fv : forall x t1 t2,
+  ~Id.FSet.In x (FV t2) -> subst x t1 t2 = t2.
+Proof.
+  intros ? ? t2 ?.
+  induction t2; simpl in *; f_equal; eauto 6.
+  - destruct (Id.eq_dec x t0).
+    + exfalso.
+      apply H.
+      apply Id.FSet.singleton_spec.
+      eauto.
+    + eauto.
+Qed.
+
+Definition subst_list s t :=
+  (fold_left (fun t s =>
+    subst (fst s) (snd s) t) s t).
+
+Lemma subst_list_Bool : forall s,
+  subst_list s Bool = Bool.
+Proof.
+  intros s.
+  induction s; simpl; eauto.
+Qed.
+
+Lemma subst_list_Fun : forall s t1 t2,
+  subst_list s (Fun t1 t2) = Fun (subst_list s t1) (subst_list s t2).
+Proof.
+  intros s.
+  induction s; intros ? ?; simpl; eauto.
+Qed.
+
+Notation unifies s t1 t2 :=
+  (subst_list s t1 = subst_list s t2).
+
+Lemma subst_preserves_unifies : forall x t0 s t,
+  unifies s (Var x) t0 ->
+  unifies s t (subst x t0 t).
+Proof.
+  intros ? ? ? t ?.
+  induction t; simpl in *; eauto.
+  - repeat rewrite subst_list_Fun.
+    f_equal; eauto.
+  - destruct (Id.eq_dec x t1); subst; eauto.
+Qed.
+
+Lemma unifies_occur : forall x t,
+  Var x <> t -> Id.FSet.In x (FV t) -> forall s, ~unifies s (Var x) t.
+Proof.
+  intros x t ? ? s Hunifies.
+  assert (Hsize : size (subst_list s t) <= size (subst_list s (Var x))) by (rewrite Hunifies; omega).
+  clear Hunifies.
+  induction t; simpl in *.
+  - destruct (Id.FSet.empty_spec H0).
+  - apply Id.FSet.union_spec in H0.
+    rewrite subst_list_Fun in *.
+    simpl in *.
+    destruct H0; [ apply IHt1 | apply IHt2 ]; eauto;
+      try (intros Hcontra; rewrite Hcontra in *);
+      omega.
+  - apply Id.FSet.singleton_spec in H0.
+    congruence.
+Qed.
