STLC/Constraint.v
@@ -1,0 +1,305 @@
+Require Import List Recdef Omega Finite_sets_facts.
+Require Id Types.
+
+Lemma Forall_map : forall X Y (P : Y -> Prop) (f : X -> Y) l,
+  Forall P (map f l) <-> Forall (fun x => P (f x)) l.
+Proof.
+  intros ? ? ? ? l.
+  split; intros H.
+  - apply Forall_forall.
+    intros ? ?.
+    Hint Resolve in_map.
+    eapply Forall_forall in H; eauto.
+  - induction l;
+    simpl;
+    inversion H;
+    eauto.
+Qed.
+
+Definition t := list (Types.t * Types.t).
+
+Notation FV c :=
+  (fold_right Id.FSet.union Id.FSet.empty
+    (map (fun p => Id.FSet.union (Types.FV (fst p)) (Types.FV (snd p))) c)).
+
+Notation size c :=
+  (fold_right plus 0 (map (fun p =>
+    Types.size (fst p) + Types.size (snd p)) c)).
+
+Notation subst x t c :=
+  (map (fun p => (Types.subst x t (fst p), Types.subst x t (snd p))) c).
+
+Notation subst_list s c :=
+  (map (fun p => (Types.subst_list s (fst p), Types.subst_list s (snd p))) c).
+
+Notation unifies s c :=
+  (Forall (fun p => Types.unifies s (fst p) (snd p)) c).
+
+Lemma subst_occur : forall x t c,
+  Id.FSet.In x (FV (subst x t c)) -> Id.FSet.In x (Types.FV t).
+Proof.
+  intros ? ? c H.
+  induction c as [| [] ]; simpl in *.
+  - destruct (Id.FSet.empty_spec H).
+  - apply Id.FSet.union_spec in H.
+    destruct H as [ H | H ].
+    + apply Id.FSet.union_spec in H.
+      Hint Resolve Types.subst_occur.
+      destruct H; eauto.
+    + eauto.
+Qed.
+
+Lemma subst_fv : forall x y t c,
+  Id.FSet.In x (FV (subst y t c)) -> Id.FSet.In x (Types.FV t) \/ Id.FSet.In x (FV c).
+Proof.
+  intros ? ? ? c H.
+  induction c as [| [] ]; simpl in *.
+  - destruct (Id.FSet.empty_spec H).
+  - apply Id.FSet.union_spec in H.
+    destruct H as [ H | H ].
+    + apply Id.FSet.union_spec in H.
+      destruct H as [ H | H ];
+      destruct (Types.subst_fv _ _ _ _ H); eauto 6.
+    + destruct (IHc H); eauto.
+Qed.
+
+Lemma subst_preserves_unifies : forall x t0 s c,
+  Types.unifies s (Types.Var x) t0 ->
+  unifies s c ->
+  unifies s (subst x t0 c).
+Proof.
+  intros ? ? ? ? ? ?.
+  apply Forall_map.
+  eapply Forall_impl; [| eauto ].
+  intros [] ?.
+  simpl in *.
+  repeat rewrite <- Types.subst_preserves_unifies;
+  eauto.
+Qed.
+
+Hint Resolve subst_preserves_unifies.
+
+Definition lt c1 c2 :=
+  (Id.FSet.cardinal (FV c1) <= Id.FSet.cardinal (FV c2)) /\
+  (Id.FSet.cardinal (FV c2) <= Id.FSet.cardinal (FV c1) -> size c1 < size c2).
+
+Lemma lt_subst : forall c x t t1 t2,
+  ~Id.FSet.In x (Types.FV t) ->
+  (t1 = t /\ t2 = Types.Var x \/ t1 = Types.Var x /\ t2 = t) ->
+  lt (subst x t c) ((t1, t2) :: c).
+Proof.
+  intros c x t ? ? Hmem Heq.
+  assert (Hcardinal : Id.FSet.cardinal (FV (subst x t c)) < Id.FSet.cardinal (FV ((t1, t2) :: c))).
+  - apply Id.FSetProperties.subset_cardinal_lt with (x := x); simpl.
+    + intros y HIn.
+      destruct (subst_fv _ _ _ _ HIn);
+      destruct Heq as [[] | []]; subst; eauto.
+    + destruct Heq as [[] | []]; subst; simpl; eauto 6.
+    + intros Hoccur.
+      apply subst_occur in Hoccur.
+      eauto.
+  - split; omega.
+Qed.
+
+Lemma lt_cons : forall p c,
+  lt c (p :: c).
+Proof.
+  intros [t] c.
+  split; simpl in *.
+  - apply Id.FSetProperties.subset_cardinal.
+    intros ? ?.
+    eauto.
+  - specialize (Types.size_gt_0 t). intros. omega.
+Qed.
+
+Lemma lt_fun : forall t11 t12 t21 t22 c',
+  lt ((t11, t21) :: (t12, t22) :: c')
+    ((Types.Fun t11 t12, Types.Fun t21 t22) :: c').
+Proof.
+  intros.
+  split; simpl.
+  - apply Id.FSetProperties.subset_cardinal.
+    intros ? H.
+    apply Id.FSet.union_spec in H.
+    destruct H as [ H | H ].
+    + apply Id.FSet.union_spec in H.
+      destruct H; eauto 7.
+    + apply Id.FSet.union_spec in H.
+      destruct H as [ H | H ].
+      * apply Id.FSet.union_spec in H.
+        destruct H; eauto 7.
+      * eauto.
+  - omega.
+Qed.
+
+Hint Resolve lt_subst lt_cons lt_fun.
+
+Lemma lt_wf : well_founded lt.
+Proof.
+  intros c.
+  remember (Id.FSet.cardinal (FV c)) as n.
+  generalize dependent c.
+  induction n as [n IHn] using lt_wf_ind.
+  intros.
+  induction c as [c IHc] using (induction_ltof1 _ (fun c => size c)).
+  subst.
+  constructor.
+  intros c' Hlt.
+  destruct Hlt as [ ? Hlt ].
+  destruct (eq_nat_dec (Id.FSet.cardinal (FV c)) (Id.FSet.cardinal (FV c'))).
+  - apply IHc; eauto.
+    apply Hlt.
+    omega.
+  - eapply IHn; eauto.
+    omega.
+Qed.
+
+Function unify c { wf lt c } :=
+  match c with
+  | nil => Some nil
+  | (t1, t2) :: c' =>
+      if Types.eq_dec t1 t2 then unify c'
+      else
+        match t1, t2 with
+        | Types.Var x, _ =>
+            if Id.FSet.mem x (Types.FV t2) then None
+            else option_map (cons (x, t2)) (unify (subst x t2 c'))
+        | _, Types.Var x =>
+            if Id.FSet.mem x (Types.FV t1) then None
+            else option_map (cons (x, t1)) (unify (subst x t1 c'))
+        | Types.Fun t11 t12, Types.Fun t21 t22 =>
+            unify ((t11, t21) :: (t12, t22) :: c')
+        | _, _ => None
+        end
+  end.
+Proof.
+  - intros. apply lt_cons.
+  - intros. apply lt_subst; eauto.
+    intros H.
+    apply Id.FSet.mem_spec in H.
+    congruence.
+  - intros. apply lt_fun.
+  - intros. apply lt_subst; eauto.
+    intros H.
+    apply Id.FSet.mem_spec in H.
+    congruence.
+  - intros. apply lt_subst; eauto.
+    intros H.
+    apply Id.FSet.mem_spec in H.
+    congruence.
+  - apply lt_wf.
+Qed.
+
+Theorem unify_sound : forall c s,
+  unify c = Some s -> unifies s c.
+Proof.
+  intros c.
+  induction c as [[| [t1 t2]] IHc] using (well_founded_induction lt_wf);
+    rewrite unify_equation;
+    intros ? Hunify.
+  - inversion Hunify.
+    eauto.
+  - destruct (Types.eq_dec t1 t2).
+    + subst.
+      eauto.
+    + destruct t1; destruct t2;
+        repeat match goal with
+        | H : context [if Id.FSet.mem ?x ?s then _ else _] |- _ =>
+            let b := fresh in
+            remember (Id.FSet.mem x s) as b;
+            destruct b;
+            [| let H' := fresh in
+               assert (H' : ~Id.FSet.In x s)
+                 by (intros H'; apply Id.FSet.mem_spec in H'; congruence) ]
+        | H : option_map (cons _) (unify ?c) = _ |- _ =>
+            let o := fresh in
+            let Heqo := fresh in
+            remember (unify c) as o eqn:Heqo;
+            symmetry in Heqo;
+            destruct o
+        | H : unify ?c = Some ?s |- _ =>
+            assert (unifies s c) by (apply IHc; eauto); clear H
+        end;
+        repeat (match goal with
+        | _ => rewrite Types.subst_list_Fun in *
+        | _ => rewrite Types.subst_notin_fv in * by eauto
+        | H : Some _ = Some _ |- _ => inversion H; clear H
+        | |- context [Id.eq_dec ?x ?y] => destruct (Id.eq_dec x y)
+        | H : ~Id.FSet.In ?x (Id.FSet.union ?s1 ?s2) |- _ =>
+            assert (~Id.FSet.In x s1) by eauto;
+            assert (~Id.FSet.In x s2) by eauto;
+            clear H
+        | |- Forall _ (_ :: _) => constructor
+        | H : Forall _ (_ :: _) |- _ => inversion H; clear H
+        | H : Forall _ (map _ _) |- _ => apply Forall_map in H
+        end; simpl in *; subst);
+        solve [ eauto | congruence ].
+Qed.
+
+Notation moregen s s' :=
+  (exists s0, forall e, Types.subst_list s e = Types.subst_list s0 (Types.subst_list s' e)).
+
+Lemma moregen_extend : forall subs x t subs',
+  Types.unifies subs (Types.Var x) t ->
+  moregen subs subs' ->
+  moregen subs ((x, t) :: subs').
+Proof.
+  intros ? x t ? ? Hmoregen.
+  destruct Hmoregen as [ s0 Hmoregen' ].
+  exists s0.
+  intros ?.
+  simpl.
+  rewrite <- Hmoregen'.
+  erewrite Types.subst_preserves_unifies; eauto.
+Qed.
+
+Theorem unify_complete : forall c s,
+  unifies s c ->
+  exists s', unify c = Some s' /\ moregen s s'.
+Proof.
+  intros c.
+  induction c as [[| [t1 t2]] IHc] using (well_founded_induction lt_wf);
+    rewrite unify_equation;
+    intros s Hunifies.
+  - exists nil.
+    simpl.
+    eauto.
+  - destruct (Types.eq_dec t1 t2).
+    + subst.
+      inversion Hunifies.
+      eauto.
+    + inversion Hunifies. subst. clear Hunifies.
+      simpl in *.
+      destruct t1; destruct t2;
+        repeat match goal with
+        | |- context [Id.FSet.mem ?x ?s] =>
+            let b := fresh in
+            let Heqb := fresh in
+            remember (Id.FSet.mem x s) as b eqn:Heqb;
+            symmetry in Heqb;
+            destruct b;
+            [ apply Id.FSet.mem_spec in Heqb;
+              exfalso;
+              eapply Types.unifies_occur; eauto
+            | let H' := fresh in
+              assert (H' : ~Id.FSet.In x s)
+                by (intros H'; apply Id.FSet.mem_spec in H'; congruence) ]
+        | |- context [unify ?c] =>
+            let H := fresh in
+            assert (H : exists s', unify c = Some s' /\ moregen s s');
+            [ apply IHc; eauto
+            | destruct H as [? [H]];
+              rewrite H ]
+        end;
+        repeat (simpl in *; match goal with
+        | H : Types.Fun _ _ = Types.Fun _ _ |- _ => inversion H; clear H
+        | _ => apply moregen_extend
+        | _ => apply subst_preserves_unifies
+        | _ => rewrite Types.subst_list_Bool in *
+        | _ => rewrite Types.subst_list_Fun in *
+        | |- exists _, Some _ = Some _ /\ _ =>
+            eexists;
+            split; [ reflexivity |]
+        end);
+        solve [ eauto | congruence ].
+Qed.
